MySQL.thy
@@ -7,7 +7,7 @@ type_synonym var = string
 datatype table = PERSON | ENROLLMENT
 datatype col = AGE | EMAIL | ID | LECTURERS | STUDENTS
 
-datatype exp = Int int 
+datatype exp = Int nat 
   | Var var 
   | Eq exp exp
   | Col col
@@ -17,76 +17,100 @@ datatype whereClause = WHERE exp
 
 datatype SQLstm = Select exp 
   | SelectFrom exp fromItem
-| SelectFromWhere exp fromItem whereClause 
-and fromItem = Table table | Subselect SQLstm
+  | SelectFromWhere exp fromItem whereClause 
+and fromItem = Table table 
+  | Subselect SQLstm
 
 fun isID :: "col \<Rightarrow> table \<Rightarrow> bool" where
-"isID ID PERSON = True " |
-"isID _ _ = False"
+"isID ID PERSON = True "
+  | "isID _ _ = False"
 
-fun execFrom :: "fromItem \<Rightarrow> persons \<Rightarrow> val" where
-"execFrom (Table _) ps  = mapPersonsToVList ps" |
-"execFrom (Subselect _) ps = VNULL"
+fun execFrom :: "fromItem \<Rightarrow> Objectmodel \<Rightarrow> val" where
+"execFrom (Table PERSON) om  = TPerson om"
+  | "execFrom (Table ENROLLMENT) om = TEnrollment om" 
+  | "execFrom (Subselect _) ps = VNULL"
 
 fun sat :: "val \<Rightarrow> exp \<Rightarrow> bool" where
 "sat v e = True"
 
+fun getAssociationEnd :: "col \<Rightarrow> Enrollment \<Rightarrow> string" where
+"getAssociationEnd STUDENTS (E students lecturers) = students"
+  | "getAssociationEnd LECTURERS (E students lecturers) = lecturers"
+
 fun proj :: "exp \<Rightarrow> val \<Rightarrow> val" where 
-"proj (Col AGE) (VPerson (P pid page pemail pstudents plecturers)) 
-= VInt page" |
-"proj (Col EMAIL) (VPerson (P pid page pemail pstudents plecturers)) 
-= VString pemail" |
-"proj (Col ID) (VPerson (P pid page pemail pstudents plecturers)) 
-= VString pid" |
-"proj (Col STUDENTS) (VPerson (P pid page pemail pstudents plecturers)) 
-= mapPersonsToVList pstudents" |
-"proj (Col LECTURERS) (VPerson (P pid page pemail pstudents plecturers)) 
-= mapPersonsToVList plecturers" |
-"proj (MySQL.Int i) v = VInt i" |
-"proj (Var var) v = VString var" |
-"proj (Eq e1 e2) v = VBool (equalVal (proj e1 v) (proj e2 v))" |
-"proj _ _ = VNULL"
+"proj (Col AGE) (VPerson (P pid page pemail)) = VInt page"
+  | "proj (Col EMAIL) (VPerson (P pid page pemail)) = VString pemail"
+  | "proj (Col ID) (VPerson (P pid page pemail)) = VString pid"
+  | "proj (MySQL.Int i) v = VInt i"
+  | "proj (MySQL.Col col) VNULL = VNULL"
+  | "proj (Var var) v = VString var" 
+  | "proj (Eq e1 e2) v = VBool (equalVal (proj e1 v) (proj e2 v))" 
+  | "proj (Col STUDENTS) (VEnrollment v) = VString (getAssociationEnd STUDENTS v)" 
+  | "proj (Col LECTURERS) (VEnrollment v) = VString (getAssociationEnd LECTURERS v)"
 
-fun isIdPerson :: "var \<Rightarrow> Person \<Rightarrow> bool" where
-"isIdPerson v (P pid page pemail pstudents plecturers) 
-= (v = pid)"
+fun ext :: "var \<Rightarrow> col \<Rightarrow> Person list \<Rightarrow> val" where
+"ext v col [] = VNULL"
+  | "ext v col (p#ps) = (if (isIdPerson v p) 
+    then (proj (Col col) (VPerson p)) 
+    else (ext v col ps))"
 
-fun ext :: "var \<Rightarrow> col \<Rightarrow> persons \<Rightarrow> val" where
-"ext v col Nil = VNULL" |
-"ext v col (p#ps) = 
-(if (isIdPerson v p) then (proj (Col col) (VPerson p)) 
-else (ext v col ps))"
+fun extElement :: "var \<Rightarrow> Person list \<Rightarrow> val" where
+"extElement v [] = VNULL"
+  | "extElement v (p#ps) = (if (isIdPerson v p) 
+    then (VPerson p)
+    else extElement v ps)"
 
-fun extElement :: "var \<Rightarrow> persons \<Rightarrow> val" where
-"extElement v Nil = VNULL" |
-"extElement v (Cons p ps) =
-(if (isIdPerson v p) then (VPerson p)
-else extElement v ps)"
+fun isAssociation :: "var \<Rightarrow> col \<Rightarrow> Enrollment \<Rightarrow> bool" where
+"isAssociation v STUDENTS (E students lecturers) = (students = v)" 
+  | "isAssociation v LECTURERS (E students lecturers) = (lecturers = v)" 
+  | "isAssociation v col _ = False"
+
+fun opposite :: "col \<Rightarrow> col" where
+"opposite STUDENTS = LECTURERS"
+  | "opposite LECTURERS = STUDENTS"
+
+(* extCol returns VList of elements standing in column col such that
+v stands in the column opposite to col *)
+fun extCol :: "var \<Rightarrow> col \<Rightarrow> Enrollment list \<Rightarrow> val list" where
+"extCol v col Nil = Nil" 
+  | "extCol v col (e#es) = (if isAssociation v (opposite col) e 
+    then (VString (getAssociationEnd col e))#(extCol v col es)
+    else extCol v col es)"
+
+(* extEnrollment returns VList of enrollments such that
+v stands in the column col *)
+fun extEnrollment :: "var \<Rightarrow> col \<Rightarrow> Enrollment list \<Rightarrow> val list" where
+"extEnrollment v col Nil = Nil" 
+  | "extEnrollment v col (e#es) = (if isAssociation v col e 
+    then  (VEnrollment e)#(extEnrollment v col es) 
+    else extEnrollment v col es)"
 
 fun filterWhere :: "val \<Rightarrow> whereClause \<Rightarrow> val" where
-"filterWhere (VList Nil) (WHERE e) = VList Nil" |
-"filterWhere (VList (Cons v vs)) (WHERE e)
-= (if sat v e 
-then (appendList v (filterWhere (VList vs) (WHERE e)))   
-else filterWhere (VList vs) (WHERE e))" |
-"filterWhere v e = v"
+"filterWhere (VList Nil) (WHERE e) = VList Nil" 
+  | "filterWhere (VList (Cons v vs)) (WHERE e) = (if sat v e 
+    then (appendList v (filterWhere (VList vs) (WHERE e)))   
+    else filterWhere (VList vs) (WHERE e))"
 
-fun select :: "val \<Rightarrow> exp \<Rightarrow> val" where
-"select VNULL (MySQL.Int i) = VList [VInt i]" |
-"select VNULL (MySQL.Var var) = VList [VString var]" |
-"select VNULL (MySQL.Eq e1 e2) = 
-VList [VBool (equalVal (select VNULL e1) (select VNULL e2))]" |
-"select VNULL (Count col) = VList [VInt 0]" |
-"select VNULL (Col col) = VNULL" |
-"select (VList Nil) exp = VList Nil" |
-"select (VList (v#vs)) exp = 
-appendList (proj exp v) (select (VList vs) exp)"
+fun select :: "val \<Rightarrow> exp \<Rightarrow> val list" where
+"select VNULL (MySQL.Int i) = [VInt i]" 
+  | "select VNULL (MySQL.Var var) = [VString var]" 
+  | "select VNULL (MySQL.Eq e1 e2) = 
+    [VBool (equalVal (VList (select VNULL e1)) (VList (select VNULL e2)))]" 
+  | "select VNULL (Col col) = [VNULL]"
+  | "select val (Count col) = [VInt (sizeValList val)]"
+  | "select (VList Nil) exp = Nil" 
+  | "select (VList (v#vs)) exp = 
+    (proj exp v) # (select (VList vs) exp)"
 
-fun exec :: "SQLstm \<Rightarrow> persons \<Rightarrow> val" where
-"exec (Select selitems) ps  = select VNULL selitems" |
-"exec (SelectFrom selitems fromItem) ps 
-= select (execFrom fromItem ps) selitems" |
-"exec (SelectFromWhere selitems fromItem whereExp) ps
-= select (filterWhere (execFrom fromItem ps) whereExp) selitems"
+fun exec :: "SQLstm \<Rightarrow> Objectmodel \<Rightarrow> val" where
+"exec (Select selitems) ps  = VList (select VNULL selitems)"
+  | "exec (SelectFrom (Count col) fromItem) ps
+    = VList [VInt (sizeValList (VList (select (execFrom fromItem ps) (Col col))))]" 
+  | "exec (SelectFrom exp fromItem) ps 
+    = VList (select (execFrom fromItem ps) exp)" 
+  | "exec (SelectFromWhere (Count col) fromItem whereExp) ps
+    = VList [VInt (sizeValList (VList (select (filterWhere (execFrom fromItem ps) whereExp) (Col col))))]" 
+  | "exec (SelectFromWhere exp fromItem whereExp) ps
+    = VList (select (filterWhere (execFrom fromItem ps) whereExp) exp)"
 
 end
