ObjectModel.thy
@@ -3,40 +3,57 @@ imports Main
 begin
 
 (* Person(id, age, email, students, lecturers) *)
-datatype Person = P string int string "Person list" "Person list"
+datatype Person = P string nat string | PNULL
 
-type_synonym persons = "Person list" 
+(* Enrollment (students, lecturers) *)
+datatype Enrollment = E string string
 
-datatype val =  VNULL | VInt int | VString string 
-  |  VBool bool | VPerson Person | VList "val list"
+datatype Objectmodel = OM "Person list" "Enrollment list"
 
-fun appendList :: "val \<Rightarrow> val \<Rightarrow> val" where
-"appendList VNULL v = v" |
-"appendList v VNULL = VNULL" |
-"appendList v (VList vs) = VList (v#vs)" |
-"appendList _ _ = VNULL"
+datatype val =  VNULL | VInt nat | VString string | VBool bool 
+  | VPerson Person | VEnrollment Enrollment 
+  | VList "val list"
+  | TPerson Objectmodel
+  | TEnrollment Objectmodel
 
-fun mapPersonsToVList :: "persons \<Rightarrow> val" where
-"mapPersonsToVList Nil = VList Nil" |
-"mapPersonsToVList (p#ps) = appendList (VPerson p) (mapPersonsToVList ps)"
+fun isIdPerson :: "string \<Rightarrow> Person \<Rightarrow> bool" where
+"isIdPerson v (P pid page pemail) = (v = pid)" |
+"isIdPerson v PNULL = False"
 
-fun isEmptyVList :: "val \<Rightarrow> bool" where 
-"isEmptyVList (VList Nil) = True" |
-"isEmptyVList _ = False"
+fun getPersonFromId :: "string \<Rightarrow> Person list \<Rightarrow> Person" where
+"getPersonFromId s [] = PNULL" |
+"getPersonFromId s (p#ps) = (if isIdPerson s p then p else (getPersonFromId s ps))"
+
+fun getPersonList :: "Objectmodel \<Rightarrow> Person list" where
+"getPersonList (OM ps es) = ps"
+
+fun getEnrollmentList :: "Objectmodel \<Rightarrow> Enrollment list" where
+"getEnrollmentList (OM ps es) = es"
+
+fun mapPersonListToValList :: "Person list \<Rightarrow> val list" where
+"mapPersonListToValList [] = []" |
+"mapPersonListToValList (p#ps) = (VPerson p)#(mapPersonListToValList ps)"
 
 fun equalVal :: "val \<Rightarrow> val \<Rightarrow> bool" where
 "equalVal (VInt i1) (VInt i2) = (i1 = i2)" |
 "equalVal (VBool b1) (VBool b2) = (b1 \<longleftrightarrow> b2)" |
 "equalVal (VString s1) (VString s2) = (s1 = s2)" |
 "equalVal (VPerson p1) (VPerson p2) = (p1 = p2)" |
-"equalVal (VList Nil) (VList Nil) = True" |
-"equalVal (VList (Cons v1 v1s)) (VList (Cons v2 v2s)) = 
-(if (equalVal v1 v2) then (equalVal (VList v1s) (VList v2s)) else False)" |
-"equalVal _ _ = False" 
+"equalVal (VList []) (VList []) = True" |
+"equalVal (VList (v1#v1s)) (VList (v2#v2s)) = 
+(if (equalVal v1 v2) then (equalVal (VList v1s) (VList v2s)) else False)"
 
-fun countVList :: "val \<Rightarrow> int" where 
-"countVList (VList Nil) = 0" |
-"countVList (VList (v#vs)) = 1 + countVList (VList vs)" |
-"countVList _ = 0"
+fun countValList :: "val list \<Rightarrow> int" where 
+"countValList [] = 0" |
+"countValList (v#vs) = 1 + countValList vs"
+
+fun appendList :: "val \<Rightarrow> val \<Rightarrow> val" where
+"appendList VNULL v = v" |
+"appendList v VNULL = VNULL" |
+"appendList v (VList vs) = VList (v#vs)"
+
+fun sizeValList :: "val \<Rightarrow> nat" where
+"sizeValList (VList []) = 0" |
+"sizeValList (VList (x#xs)) = Suc (sizeValList (VList xs))"
 
 end
