MyMain.thy
@@ -2,54 +2,59 @@ theory MyMain
   imports Main MyOCL MySQL
 begin
 
-(* self = caller *)
-lemma "\<forall> self caller om. eval (MyOCL.Eq (MyOCL.Var self) (MyOCL.Var caller)) om 
+lemma lem4 : "filterWhere (TEnrollment om) 
+(WHERE (MySQL.Eq (Col col) (MySQL.Var var)))
+= VList (extEnrollment var col (getEnrollmentList om))"
+  sorry
+
+lemma lem1 : "filterWhere (TPerson om) 
+(WHERE (MySQL.Eq (Col MySQL.ID) (MySQL.Var var)))
+= VList [extElement var (getPersonList om)]"
+  sorry
+
+lemma lem2 : "proj (Col col) (extElement v ps) 
+= ext v col ps"
+  apply (induct ps)
+   apply simp_all
+  done
+
+(* self = caller \<equiv> SELECT self = caller *)
+lemma "eval (MyOCL.Eq (MyOCL.Var self) (MyOCL.Var caller)) om 
 = exec (Select (MySQL.Eq (MySQL.Var self) (MySQL.Var caller))) om"
   apply auto
   done
 
-lemma lem1 : "filterWhere (mapPersonsToVList persons) 
-(WHERE (MySQL.Eq (Col MySQL.ID) (MySQL.Var var)))
-= VList [extElement var persons]"
-  sorry
-
-lemma lem4 : "filterWhere (mapPersonsToVList persons) 
-(WHERE (MySQL.Eq (Col col) (MySQL.Var var)))
-= VList [extElement var persons]"
-  sorry
-
-lemma lem2 : "proj (Col col) (extElement v om) 
-= ext v col om"
-  apply (induct om)
-   apply simp_all
-  done
- 
-(* self.age = 30 *)
+(* self.age = 30 \<equiv> SELECT age = 30 FROM Person WHERE id = self *)
 lemma " eval (MyOCL.Eq (MyOCL.Att self MyOCL.AGE) (MyOCL.Int 30)) om
 = exec (SelectFromWhere (MySQL.Eq (MySQL.Col (MySQL.AGE)) (MySQL.Int 30))
 (Table PERSON)
 (WHERE (MySQL.Eq (MySQL.Col (MySQL.ID)) (MySQL.Var self)))) om" 
-  apply auto
+  apply (auto)
    apply (simp_all add: lem1 lem2)
   done
 
-(* self.lecturers *)
-lemma lem3 : "eval (MyOCL.As self MyOCL.LECTURERS) om
+(* self.lecturers \<equiv> SELECT lecturers FROM Enrollment WHERE students = self *)
+lemma "eval (MyOCL.As self MyOCL.LECTURERS) (OM ps es)
 = exec (SelectFromWhere (MySQL.Col MySQL.LECTURERS) 
 (Table ENROLLMENT)
-(WHERE (MySQL.Eq (MySQL.Col (MySQL.STUDENTS)) (MySQL.Var self)))) om"
-  apply auto
-  apply (simp add: lem4 lem2)
+(WHERE (MySQL.Eq (MySQL.Col (MySQL.STUDENTS)) (MySQL.Var self)))) (OM ps es)"
+    apply auto
+    apply (simp add: lem4)
+    apply (induct es)
+   apply auto
+  done
 
-
-(*
-(* self.lecturers\<rightarrow>size() *)
-lemma "eval (MyOCL.Size (MyOCL.As self MyOCL.LECTURERS)) om
+(* self.lecturers\<rightarrow>size() \<equiv> SELECT COUNT(lecturers) FROM Enrollment WHERE students = self *)
+lemma "eval (MyOCL.Size (MyOCL.As self MyOCL.LECTURERS)) (OM ps es)
 = exec (SelectFromWhere (MySQL.Count MySQL.LECTURERS) 
 (Table ENROLLMENT)
-(WHERE (MySQL.Eq (MySQL.Col (MySQL.STUDENTS)) (MySQL.Var self)))) om"
-  sorry
-*)
+(WHERE (MySQL.Eq (MySQL.Col (MySQL.STUDENTS)) (MySQL.Var self)))) (OM ps es)"
+  apply auto
+  apply(simp add: lem4)
+  apply (induct es)
+   apply auto
+  done  
+
 end
 
   
